finish week05 except week04 Sheet3

my_exercises/Week05 Inductive Predicates/HW4.lean
@@ -13,17 +13,30 @@ def isEven (n :ℕ) : Prop := ∃k, n = 2*k
 
 -- Your AllEven must use isEven function above
 inductive AllEven : List ℕ → Prop
+  | nil : AllEven []
+  | single (a : ℕ) : isEven a → AllEven [a]
+  | cons (a : ℕ) (l : List ℕ) : isEven a → (AllEven l → AllEven (a::l))
 
 -- Prove that your AllEven predicate is equivalent to checking if every element in the list is even.
 -- Let's split into two parts
 
 -- # Part 1
-theorem Problem1_1 (l : List ℕ)  :
-  AllEven l → ∀ n ∈ l, isEven n := by sorry
+theorem Problem1_1 (l : List ℕ) : AllEven l → ∀ n ∈ l, isEven n := by
+  intro h_AE_l n h_n_l
+  induction' l
+  · contradiction
+  · simp_all
+    cases h_n_l
+    -- # Question: how to proceed step-by-step by analysing the `AllEven(head::tail)` of `h_AE_l`?
+    · grind [AllEven]
+    · grind [AllEven]
 
 -- # Part 2
-theorem Problem1_2 (l : List ℕ)  :
-  (h : ∀ n ∈ l, isEven n) → AllEven l := by sorry
+theorem Problem1_2 (l : List ℕ) : (h : ∀ n ∈ l, isEven n) → AllEven l := by
+  intro h_even_n
+  induction' l
+  · exact AllEven.nil
+  · grind [AllEven]
 
 -- # Sorted
 -- We will use the following version of Sorted
@@ -38,16 +51,40 @@ inductive Sorted: List ℕ  → Prop
 
 -- # Problem 2: Prove that a list of length at most 1 is sorted.
 def len : List ℕ → ℕ
-| []     =>  0
+| []      => 0
 | _ :: xs => 1 + len xs
 
-theorem Problem2 (l : List ℕ) (h: len l ≤ 1): Sorted l := by sorry
-
+theorem Problem2 (l : List ℕ) (h: len l ≤ 1): Sorted l := by
+  -- cases l with
+  -- | nil => exact Sorted.nil
+  -- | cons a l_tail =>
+  --   cases l_tail with
+  --   | nil => exact Sorted.single a
+  --   | cons b l_rest =>
+  --     simp [len] at h
+  cases l
+  · exact Sorted.nil
+  · cases tail
+    · exact Sorted.single head
+    -- · simp [len] at h
+    · simp only [len] at h; simp at h
 
 -- # Problem 3: Prove basic properties of Sorted
-theorem Problem3_1 {x : ℕ} {xs : List ℕ} (hxs : Sorted (x :: xs)) : Sorted xs := by sorry
-theorem Problem3_2 {x y : ℕ} {t : List ℕ} (hsort : Sorted (x :: y :: t)) : y.MinOfList t := by sorry
+theorem Problem3_1 {x : ℕ} {xs : List ℕ} (hxs : Sorted (x :: xs)) : Sorted xs := by
+  generalize h_eq : x::xs = l
+  replace hxs : Sorted l := by rwa [← h_eq]
+  -- have hxs_eq : Sorted l := by rwa [← h_eq]
+  induction' hxs generalizing xs x
+  all_goals
+  grind [Sorted]
 
+theorem Problem3_2 {x y : ℕ} {t : List ℕ} (hsort : Sorted (x :: y :: t)) : y.MinOfList t := by
+  generalize h_eq : x::y::t = l
+  replace hxyt : Sorted l := by rwa [← h_eq]
+  -- have hxs_eq : Sorted l := by rwa [← h_eq]
+  induction' hxyt generalizing x y t
+  all_goals
+  grind [Sorted, Nat.MinOfList]
 
 -- # Problem 4: Alternate Definitions of Sorted
 -- Consider the following inductive predicate
@@ -58,7 +95,28 @@ inductive Sorted2: List ℕ  → Prop
 
 -- Prove that Sorted2 is equivalent to Sorted
 -- You may find `ext` tactic useful
-theorem Problem4 : Sorted2 = Sorted := by sorry
+theorem Problem4 : Sorted2 = Sorted := by
+  ext
+  constructor
+  · intro h_s2
+    induction' x
+    · exact Sorted.nil
+    · generalize h_eq : head::tail = l
+      replace h_s2 : Sorted2 l := by rwa [h_eq] at h_s2
+      induction h_s2 generalizing head tail
+      all_goals grind [Sorted2, Sorted]
+  -- symmetrical
+  · intro h_s2
+    induction' x
+    · exact Sorted2.nil
+    · generalize h_eq : head::tail = l
+      replace h_s2 : Sorted l := by rwa [h_eq] at h_s2
+      induction h_s2 generalizing head tail
+      all_goals grind [Sorted2, Nat.MinOfList]
+      -- · grind
+      -- · grind [Sorted2]
+      -- · grind [Sorted2]
+      -- · grind [Nat.MinOfList, Sorted2]
 
 -- # Problem 5: Binary Tree
 -- Consider the following version of BinaryTree
@@ -81,6 +139,25 @@ inductive Complete : BinaryTree  → Prop
       (hiff : l = BinaryTree.nil ↔ r = BinaryTree.nil) :
     Complete (BinaryTree.node l key r)
 
+theorem mirror_nil_iff (r : BinaryTree): mirror r = BinaryTree.nil ↔ r = BinaryTree.nil := by
+  induction' r
+  · rw [mirror]
+  · rw [mirror]
+    simp only [reduceCtorEq]
+
 -- Prove that if a mirror of t is complete then t is complete
-theorem Problem5:
-    ∀t : BinaryTree, Complete (mirror t) → Complete t := by sorry
+theorem Problem5: ∀t : BinaryTree, Complete (mirror t) → Complete t := by
+  intro t
+  induction' t
+  · simp [mirror]
+  · intro h_p
+    rw [mirror] at h_p
+    cases h_p
+    apply Complete.node
+    · simp [hr] at left_ih; exact left_ih
+    · simp [hl] at right_ih; exact right_ih
+    -- # Is there a way to transform both sides of the goal into `hiff`?
+    -- # the left-hand-side is easy by rw, which doen't work on the right-hand-side
+    · rw [mirror_nil_iff, mirror_nil_iff] at hiff
+      symm
+      exact hiff
