my_exercises/Week05 Inductive Predicates/Exercise.lean
@@ -3,24 +3,63 @@ import Mathlib.Tactic -- imports all of the tactics in Lean's maths library
 set_option autoImplicit false
 set_option tactic.hygienic false
 
-
 -- # Exercise: Define IsPalindrome
 -- This should be true if and only if it can be read in forward and reverse direction
 -- e.g., 'a', 'aba', 'aabbcbbaa'
 
 inductive IsPalindrome {α : Type} : List α → Prop
---  | nil :  ??
---  | single (a : α) :  ??
---  | cons_eq (a : α) (l : List α) :  ??
+ | nil : IsPalindrome []
+ | single (a : α) : IsPalindrome [a]
+ | cons_eq (a : α) (l : List α) : (IsPalindrome l) → IsPalindrome (a::l ++ [a])
 
 theorem IsPalindrome_imp_eq_reverse {α : Type} (l : List α) :
-  IsPalindrome l → l = List.reverse l := by sorry
+  IsPalindrome l → l = List.reverse l := by
+  intro h
+  induction' h
+  · simp only [List.reverse_nil]
+  · simp only [List.reverse_cons, List.reverse_nil, List.nil_append]
+  · simpa
+  -- # Alternative 1:
+  -- · simp only [
+  --     List.cons_append, List.reverse_cons, List.reverse_append, List.reverse_nil,
+  --     List.nil_append, List.cons.injEq, List.append_cancel_right_eq, true_and
+  --   ]; assumption
+  -- # Alternative 2:
+  -- · calc
+  --     a :: l_1 ++ [a]
+  --       = a :: l_1.reverse ++ [a] := by rw [← a_ih]
+  --     _ = [a] ++ l_1.reverse ++ [a] := by
+  --       simp only [List.cons_append, List.nil_append]
+  --     _ = [a].reverse ++ l_1.reverse ++ [a].reverse := by
+  --       simp only [List.cons_append, List.nil_append, List.reverse_cons, List.reverse_nil]
+  --     _ = (a :: l_1 ++ [a]).reverse := by
+  --       simp only [List.reverse_cons, List.reverse_nil, List.nil_append, List.cons_append, List.reverse_append]
 
+-- Challenging one :)
 theorem IsPalindrome_pmi_eq_reverse {α : Type} (l : List α) :
-  l = List.reverse l → IsPalindrome l  := by sorry
+  l = List.reverse l → IsPalindrome l  := by
+  intro h_p
+  induction' l with a as ih
+  · exact IsPalindrome.nil
+  · cases as with
+    | nil =>
+      -- l = [a]
+      exact IsPalindrome.single a
+    | cons b bs =>
+      -- l = a :: b :: bs
+      sorry
 
-theorem IsPalindrome_reverse {α : Type} (l : List α) (h: IsPalindrome l) :
-   IsPalindrome l.reverse  := by sorry
+theorem IsPalindrome_reverse {α : Type} (l : List α) (h: IsPalindrome l) : IsPalindrome l.reverse  := by
+  induction' h
+  · simp only [List.reverse_nil]
+    exact IsPalindrome.nil
+  · simp only [List.reverse_cons, List.reverse_nil, List.nil_append]
+    exact (IsPalindrome.single a)
+  · rw [← IsPalindrome_imp_eq_reverse]
+  -- · rw [← IsPalindrome_imp_eq_reverse (a :: l_1 ++ [a])]
+    all_goals
+    apply IsPalindrome.cons_eq
+    exact a_1
 
 -- # Exercise: Binary Tree, Mirror and Complete Binary Tree
 -- Define BinaryTree as follows
@@ -29,17 +68,34 @@ inductive BinaryTree
   | nil
   | node (left : BinaryTree) (key : ℕ) (right : BinaryTree)
 
+#check BinaryTree
+#check BinaryTree.nil
+#check BinaryTree.node
+
 -- Define mirror operation as reversing the tree
 def mirror : BinaryTree → BinaryTree
   | BinaryTree.nil        => BinaryTree.nil
   | BinaryTree.node l key r => BinaryTree.node (mirror r) key (mirror l)
 
 --  Prove that mirror of mirror of a tree is the tree itself.
-theorem mirror_mirror (t : BinaryTree) :
-    mirror (mirror t) = t := by sorry
+theorem mirror_mirror (t : BinaryTree) : mirror (mirror t) = t := by
+  -- cases t
+  -- · rw [mirror, mirror]
+  -- · rw [mirror, mirror]
+  --   simp only [BinaryTree.node.injEq, true_and]
+  --   constructor
+  --   all_goals
+  --   rw [mirror_mirror]
+  fun_induction mirror t
+  · rw [mirror]
+  · grind [mirror]
 
 --  Prove that mirror of mirror of a tree is the tree itself.
-theorem mirror_nil_iff (r : BinaryTree): mirror r = BinaryTree.nil ↔ r = BinaryTree.nil := by sorry
+theorem mirror_nil_iff (r : BinaryTree): mirror r = BinaryTree.nil ↔ r = BinaryTree.nil := by
+  induction' r
+  · rw [mirror]
+  · rw [mirror]
+    simp only [reduceCtorEq]
 
 -- A binary tree is complete if every node has either two non-empty subtrees or two empty subtrees.
 -- We can define it using inductive predicate as follows.
@@ -52,6 +108,15 @@ inductive Complete : BinaryTree  → Prop
     Complete (BinaryTree.node l key r)
 
 -- Prove that if t is complete then its mirroring is also complete.
-theorem complete_mirror  (t : BinaryTree)
-      (ht : Complete t) :
-    Complete (mirror t) := by sorry
+theorem complete_mirror  (t : BinaryTree) (ht : Complete t) :
+  Complete (mirror t) := by
+  induction' ht
+  · rw [mirror]
+    exact Complete.leaf
+  · rw [mirror]
+    apply Complete.node
+    · exact hr_ih
+    · exact hl_ih
+    · rw [mirror_nil_iff, mirror_nil_iff]
+      symm
+      exact hiff
