my_exercises/Week05 Inductive Predicates/Sheet1_InductivePredicate.lean
@@ -4,7 +4,8 @@ set_option autoImplicit false
 set_option tactic.hygienic false
 
 --# Inductive Predicate
--- We have seen inductive types in the previous class. Today, we cover the concept of inductive predicate.
+-- We have seen `inductive types` in the previous class (`Week04 -> Sheet2`).
+-- Today, we cover the concept of `inductive predicate`.
 -- Inductive predicate is a proposition that is defined inductively which Lean supports.
 -- Let's start with a toy example
 
@@ -13,8 +14,6 @@ set_option tactic.hygienic false
   * 0 is even
   * ∀ n : ℕ, if n is even then n + 2 is even
 -/
-@[simp] def evenFun (n :ℕ ) : Prop := ∃ k, n = 2*k
-
 inductive IsEven : ℕ → Prop
 | zero : IsEven 0
 | plus_two (n:ℕ): IsEven n → IsEven (n+2)
@@ -29,12 +28,12 @@ example: IsEven 4 := by
   apply IsEven.plus_two
   exact .zero
 
-
 /-!  New Tactics for inductive predicate
-  `cases h` -- deconstruct the proof `h : IsEven n` into all possible cases `h` can be constructed using introduction rules.
-        -- Intuitively, `cases h` where `h : IsEven n` allows us to prove that
-        -- for every constructor that an element can be produced, the goal can be proved.
-        -- It breaks down into cases based on the constructor and match it to the goal.
+  `cases h`
+  -- deconstruct the proof `h : IsEven n` into all possible cases `h` can be constructed using introduction rules.
+  -- Intuitively, `cases h` where `h : IsEven n` allows us to prove that
+  * for every constructor that an element can be produced, the goal can be proved.
+  * It breaks down into cases based on the constructor and match it to the goal.
 -/
 
 example: ¬ (IsEven 3) := by
@@ -49,7 +48,9 @@ example: ¬ (IsEven 3) := by
 -- If we want to prove IsEven n for all n, we use (rule) induction.
 -- Given an hypotehsis `h : IsEven n`, and the goal is `⊢ P n`.
 -- We invoke `induction' h` and obtain two subgoals: `IsEven.zero` and `IsEven.plus_two`
--- This is called Rule Induction.
+-- This is called `Rule Induction`.
+
+@[simp] def evenFun (n : ℕ) : Prop := ∃ k, n = 2*k
 
 theorem soundness_isEven (n:ℕ ):  IsEven n → evenFun n := by
   intro h
@@ -68,21 +69,6 @@ theorem soundness_isEven (n:ℕ ):  IsEven n → evenFun n := by
 -- case `IsEven.plus_two`. In this case, `h: IsEven (n+2)` is generated from `IsEven n`,
 --                         we have  to `P (n)` and prove `P (n+2)`
 
-inductive IsEven2 : ℕ → Prop
-| zero : IsEven2 0
-| plus_two (n:ℕ): IsEven2 n → IsEven2 (n+4)
-
--- Exercise 1.1
-theorem soundness_IsEven2 (n:ℕ ):  IsEven2 n → evenFun n := by
-  intro h
-  induction' h
-  · simp [evenFun]
-  · simp_all only [evenFun]
-    obtain ⟨ k, hk ⟩ := a_ih
-    use k+2
-    rw [hk]
-    omega
-
 -- Do it together
 theorem completeness_isEven (n : ℕ): evenFun n → IsEven n := by
   intro h
@@ -95,31 +81,52 @@ theorem completeness_isEven (n : ℕ): evenFun n → IsEven n := by
   · rw [Nat.mul_add_one 2 n]
     exact IsEven.plus_two (2 * n) ih
 
+
+inductive IsEven2 : ℕ → Prop
+| zero : IsEven2 0
+| plus_two (n:ℕ): IsEven2 n → IsEven2 (n+4)
+
+#check IsEven2.zero
+#check IsEven2.plus_two
+
+-- Exercise 1.1
+theorem soundness_IsEven2 (n:ℕ ):  IsEven2 n → evenFun n := by
+  intro h
+  induction' h
+  · simp [evenFun]
+  · simp_all only [evenFun]
+    obtain ⟨ k, hk ⟩ := a_ih
+    use k+2
+    rw [hk]
+    omega
+
 -- Exercise 1.2
 theorem incompleteness_isEven2 : ∃ n, evenFun n ∧ ¬ IsEven2 n := by
   use 2
   simp [evenFun]
-  by_contra h
-  cases h
-
+  by_contra!
+  cases this
+  -- by_contra h
+  -- cases h
 
 /- Summary
 -- By analogy, the proof strategy for inductive predicates is similar to that of the disjunction.
--- h: P ∨ Q    -- `cases h` will deconstruct `h` into  two cases `h: P` and `h: Q` to prove the goal separately
--- h: IsEven n -- `cases h` will deconstruct `h` into cases that `h` can be proved by the constructors.
-               -- `induction h` is similar to `cases h`, but we obtain inductive hypothesis to prove the inductive cases.
-
--- ⊢ P ∨ Q     -- apply `inl: P` or apply `inr: Q` --> this simplifies to proving P or proving Q.
--- ⊢ IsEven n  -- apply `IsEven.zero: IsEven 0` or apply `IsEven.plus_two: IsEven n → IsEven (n+2)`.
+-- `h: P ∨ Q`    -- `cases h` will deconstruct `h` into  two cases `h: P` and `h: Q` to prove the goal separately
+-- `h: IsEven n` -- `cases h` will deconstruct `h` into cases that `h` can be proved by the constructors.
+                 -- `induction h` is similar to `cases h`, but we obtain inductive hypothesis to prove the inductive cases.
+-- `⊢ P ∨ Q`     -- apply `inl: P` or apply `inr: Q` --> this simplifies to proving P or proving Q.
+-- `⊢ IsEven n`  -- apply `IsEven.zero: IsEven 0` or apply `IsEven.plus_two: IsEven n → IsEven (n+2)`.
 -/
 
 
 -- # Challenges for induction proofs
 -- The arguments for inductive predicates evolves throughout the induction.
--- we can apply `induction h` on h: Even n. However, we cannot apply `induction h` on h: Even (n+1) because in Lean (n+1) is not a variable.
+-- we can apply `induction h` on `h: Even n`. However, we cannot apply `induction h` on `h: Even (n+1)`
+-- because in Lean (n+1) is not a variable.
+
 -- Example
 
--- generalize, replace, rwa tactics
+-- `generalize`, `replace`, `rwa` tactics
 example (m: ℕ) (h: IsEven (m+2)) : IsEven m := by
 
   -- induction h
@@ -129,6 +136,7 @@ example (m: ℕ) (h: IsEven (m+2)) : IsEven m := by
   generalize h_eq: (m+2) = k
 
   replace h: IsEven k := by rwa [← h_eq]
+    -- rw [← h_eq]; assumption
   induction' h
   · aesop
   · aesop
