my_exercises/Week05 Inductive Predicates/Sheet2_SortedProposition.lean
@@ -7,7 +7,7 @@ set_option tactic.hygienic false
 @[simp,grind] def Nat.MinOfList (a :ℕ ) (t: List ℕ) : Prop := ∀ y ∈ t, a ≤ y
 
 -- Let's discuss in English
--- How do define inductively of sortedness
+-- How to define inductively of sortedness
 
 -- inductive predicate
 inductive Sorted: List ℕ  → Prop
@@ -29,17 +29,17 @@ example: Sorted [1] := by
 -- # Example
 example: Sorted [1,2,3] := by
   apply Sorted.cons
-  omega
-  apply Sorted.cons
-  omega
-  exact Sorted.single 3
+  · omega
+  · apply Sorted.cons
+    · omega
+    · exact Sorted.single 3
 
 -- # Example
 example: ¬ Sorted [20,3,1] := by
   by_contra!
   cases this
-  omega
-  aesop
+  · omega
+  · aesop
 
 -- # Example
 example: ¬ Sorted [1,3,2] := by
@@ -58,23 +58,42 @@ example: ¬ Sorted [1,3,2] := by
 theorem sorted_min {x : ℕ} {xs : List ℕ} (hxs : Sorted (x :: xs)) :  x.MinOfList xs  := by
   cases hxs
   · simp
-  · simp only [Nat.MinOfList, List.mem_cons, forall_eq_or_imp]
+  · simp only [Nat.MinOfList]
+    simp only [List.mem_cons]
+    simp only [forall_eq_or_imp]
     constructor
+    -- about `constructor`: ..\Week01 Lean4 Basic Tactics\Sheet1_BasicLogic.lean
     · exact a_1
     · apply sorted_min at a_2
       grind
+      -- about `grind`: ..\Week03 Calculation and Induction\Sheet0_Calculation.lean
   · exact a_1
 
 -- # Exercise 5.1: Proof by induction
-theorem sorted_min' {x : ℕ} {xs : List ℕ} (hxs : Sorted (x :: xs)) :  x.MinOfList xs  := by sorry
+theorem sorted_min' {x : ℕ} {xs : List ℕ} (hxs : Sorted (x :: xs)) :  x.MinOfList xs  := by
+  generalize h_eq : x::xs = l
+  replace hxs : Sorted l := by rwa [← h_eq]
+  -- have hxs_eq : Sorted l := by rwa [← h_eq]
+  induction' hxs generalizing xs x
+  all_goals grind
 
 -- # Exercise 5.2
-theorem sorted_is_preserved_by_min_cons {a : ℕ} {t : List ℕ} (hmin : a.MinOfList t) (ht : Sorted t) : Sorted (a :: t) := by sorry
+theorem sorted_is_preserved_by_min_cons {a : ℕ} {t : List ℕ} (hmin : a.MinOfList t) (ht : Sorted t) : Sorted (a :: t) := by
+  exact Sorted.cons_min a t hmin ht
 
 -- # Exercise 5.3
--- Define `merge` function that takes two sorted lists and ouputs a sorted list
+-- Define `merge` function that takes two `sorted lists` and ouputs a sorted list
 -- merge [1, 5, 8] [2, 4, 9] = [1, 2, 4, 5, 8, 9]
 -- merge [10,20] [] = [10, 20]
 -- merge [2, 4, 4, 8] [1, 5, 8, 9] = [1, 2, 4, 4, 5, 8, 8, 9]
 
-def merge: List ℕ → List ℕ → List ℕ := sorry
+def merge: List ℕ → List ℕ → List ℕ
+  | xs, [] => xs
+  | [], ys => ys
+  | x::xs, y::ys =>
+    if x ≤ y then x::(merge xs (y::ys))
+    else y::(merge (x::xs) ys)
+
+#eval merge [1, 5, 8] [2, 4, 9]
+#eval merge [10,20] []
+#eval merge [2, 4, 4, 8] [1, 5, 8, 9]
